Change bind to choice, refine race definition/detection

reduce/ProcessRewrite.v
@@ -13,8 +13,8 @@ Section Process.
   Context {T : Type}.
   Context {eq_dec_T : forall (t1 t2 : T), {t1 = t2}+{t1 <> t2}}.
   Definition pid := nat.
-  Inductive SetVar :=
-    | X : nat -> SetVar.
+  Inductive Var :=
+    | X : nat -> Var.
   Inductive MuVar :=
     | L : nat -> MuVar.
   Definition eq_dec_pid := PeanoNat.Nat.eq_dec. 
@@ -22,9 +22,10 @@ Section Process.
   Inductive PidClass : Type :=
   | p_none : PidClass
   | p_sng  : pid -> PidClass
-  | p_set  : SetVar -> PidClass.
+  | p_var  : Var -> PidClass
+  | p_set  : Var -> PidClass.
   
-  Definition eqb_setvar (xs ys : SetVar) : bool :=
+  Definition eqb_var (xs ys : Var) : bool :=
     match (xs, ys) with
       | (X xs, X ys) => Nat.eqb xs ys
     end.
@@ -33,27 +34,29 @@ Section Process.
     match p, q with
       | p_none, p_none => true
       | p_sng p', p_sng q' => Nat.eqb p' q'
-      | p_set ps, p_set qs => eqb_setvar ps qs
+      | p_set ps, p_set qs => eqb_var ps qs
+      | p_var x, p_var y => eqb_var x y 
       | _,_ => false
     end.
         
   Definition eq_dec_pidclass : forall (p q : PidClass), {p=q}+{p<>q}.
   Proof. repeat decide equality. Qed.
   
-  Lemma eqb_pidclass_eq : 
-    forall (p q : PidClass),
-      eqb_pidclass p q = true <-> p = q.
-  Proof.
-    intros.
-    destruct (eq_dec_pidclass p q). subst.
-    split; intros. reflexivity. 
-    destruct q. reflexivity. simpl. induction p; auto.
-    simpl. destruct s. unfold eqb_setvar. induction n; auto.
-    destruct p; destruct q; split; intros; try inversion H; try congruence.
-    apply PeanoNat.Nat.eqb_eq in H1. subst. reflexivity.
-    destruct s; destruct s0.
-    apply PeanoNat.Nat.eqb_eq in H1. subst. reflexivity.
-  Qed. 
+  (* Lemma eqb_pidclass_eq :  *)
+  (*   forall (p q : PidClass), *)
+  (*     eqb_pidclass p q = true <-> p = q. *)
+  (* Proof. *)
+  (*   intros. *)
+  (*   destruct (eq_dec_pidclass p q). subst. *)
+  (*   split; intros. reflexivity.  *)
+  (*   destruct q. reflexivity. simpl. induction p; auto. *)
+    
+  (*   simpl. destruct s. unfold eqb_setvar. induction n; auto. *)
+  (*   destruct p; destruct q; split; intros; try inversion H; try congruence. *)
+  (*   apply PeanoNat.Nat.eqb_eq in H1. subst. reflexivity. *)
+  (*   destruct s; destruct s0. *)
+  (*   apply PeanoNat.Nat.eqb_eq in H1. subst. reflexivity. *)
+  (* Qed.  *)
 
   Definition M := (T * PidClass)%type.
 
@@ -68,19 +71,20 @@ Section Process.
     
   Inductive Stmt : Type :=
   | s_skip  : Stmt
-  | s_bind  : PidClass -> Stmt -> Stmt
   | s_send  : PidClass -> M -> Stmt
   | s_recv  : M -> Stmt
-  | s_recv_l: PidClass -> list (M * Stmt) -> Stmt
+  | s_recv_l: list (M * Stmt) -> Stmt
+  | s_recv_x: (T * Var) -> Stmt -> Stmt
+  (* | s_int_ch : Stmt -> Stmt -> Stmt *)
+  (* | s_ext_ch : Stmt -> Stmt -> Stmt *)
   | s_seq   : Stmt -> Stmt -> Stmt
-  | s_iter  : SetVar -> Stmt -> Stmt
+  | s_iter  : Var -> Stmt -> Stmt
   | s_loop  : MuVar -> Stmt -> Stmt
   | s_var   : MuVar -> Stmt
   (* These statements below never appear in original programs *)
   | s_loop_body : MuVar -> Stmt -> Stmt
   | s_loop_end  : MuVar -> Stmt -> Stmt.
 
-  
   Definition Process := (PidClass * Stmt)%type.
   Definition Config := list Process.
   
@@ -91,23 +95,33 @@ Section Process.
       | (_, [])    => c
       | (S n, ps'::cs') => ps' :: update_nth cs' n ps
     end.
-  
-  Fixpoint set_in (xs : SetVar) (s : Stmt) :=
+ 
+  Definition set_in_msg (xs : Var) (m : M) :=
+    match m with
+      | (_, p_set xs') => xs = xs'
+      | _ => False
+    end.
+
+  Fixpoint set_in (xs : Var) (s : Stmt) :=
     match s with
-      | s_int_ch s t => set_in xs s \/ set_in xs t
-      | s_ext_ch s t => set_in xs s \/ set_in xs t
-      | s_bind _ t => set_in xs t
+      (* | s_int_ch s t => set_in xs s \/ set_in xs t *)
+      (* | s_ext_ch s t => set_in xs s \/ set_in xs t *)
+      | s_recv_l ss => fold_left (fun i s => i \/ 
+                                             set_in_msg xs (fst s) \/ 
+                                             set_in xs (snd s)) ss False
+      (* | s_bind _ t => set_in xs t *)
       | s_seq t u => set_in xs t \/ set_in xs u
-      | s_send (p_set xs') (_, p_set xs'') => xs = xs' \/ xs = xs''
-      | s_recv (_, p_set xs') => xs = xs'
+      | s_send (p_set xs') m => xs = xs' \/ set_in_msg xs m
+      | s_recv m => set_in_msg xs m
+      | s_recv_x (t,x') u => x' = xs \/ set_in xs u
       | s_iter _ t => set_in xs t
       | s_loop _ t => set_in xs t
       | s_loop_body _ t => set_in xs t
       | s_loop_end _ t => set_in xs t
-      | _ => False
+      | _ => True
     end.
   
-  Axiom measure : SetVar -> nat.
+  Axiom measure : Var -> nat.
 
   Inductive EqStmt : Stmt -> Stmt -> Prop :=
     | stmt_refl : 
@@ -138,7 +152,7 @@ Section Process.
             (s_seq (s_loop_body X (s_var X)) (s_loop X s))
             (s_loop X s)
     | stmt_set : 
-        forall (s : Stmt) (xs xs' : SetVar),
+        forall (s : Stmt) (xs xs' : Var),
           ~ set_in xs s -> EqStmt (s_iter xs s) (s_iter xs' s).
   
   Hint Constructors EqStmt : eqstmt.
@@ -158,7 +172,7 @@ Section Process.
   Qed.
    
   Inductive Context :=
-  | Mult : SetVar -> Context
+  | Mult : Var -> Context
   | Loop : MuVar -> Context.
 
   Fixpoint head_stmt' s stk :=
@@ -203,14 +217,40 @@ Section Process.
   Definition eq_dec_m : forall m1 m2 : M, {m1=m2}+{m1<>m2}.
   Proof. repeat decide equality. Qed.
   
-  Definition elim ps qs :=
-    match (get_stmt ps, get_stmt qs) with
-      | (s_send q m, s_recv m') => 
-        if (eq_dec_m m m') then eqb_pidclass q (get_pid qs) else false
-      | (s_recv m', s_send p m) => 
-        if (eq_dec_m m m') then eqb_pidclass p (get_pid ps) else false
-      | _ => false
+  Definition subst_pid p q p' :=
+    if eqb_pidclass p p' then q else p'.
+    (* match (p, p') with *)
+    (*   | (p_sng p, p_sng pid') => if eq_dec_pid p pid' then q else p' *)
+    (*   | _ => p' *)
+    (* end. *)
+  
+  Fixpoint subst_stmt p q s :=
+    match s with
+      | s_skip => s_skip
+      | s_send p' m => s_send (subst_pid p q p') (subst_pid_m p q m)
+      | s_recv m => s_recv (subst_pid_m p q m)
+      | s_seq s' t' => s_seq (subst_stmt p q s') (subst_stmt p q t')
+      | _ => s
     end.
+  
+  Fixpoint inst_stmt (x : Var) (c : list PidClass) (s : Stmt) :=
+    match s with
+      | s_recv_x (t,x') s' =>
+        s_recv_l (map (fun p => ((t,p), subst_stmt (p_var x) p s')) c)
+      | s_seq t u => s_seq (inst_stmt x c t) (inst_stmt x c u)
+      | s_iter xs s => s_iter xs (inst_stmt x c s)
+      | s_loop y s => s_loop y (inst_stmt x c s)
+      | _ => s
+    end.
+  
+  (* Definition elim ps qs := *)
+  (*   match (get_stmt ps, get_stmt qs) with *)
+  (*     | (s_send q m, s_recv m') =>  *)
+  (*       if (eq_dec_m m m') then eqb_pidclass q (get_pid qs) else false *)
+  (*     | (s_recv m', s_send p m) =>  *)
+  (*       if (eq_dec_m m m') then eqb_pidclass p (get_pid ps) else false *)
+  (*     | _ => false *)
+  (*   end. *)
   
   Definition Elim ps qt :=
     match (get_stmt ps, get_stmt qt) with
@@ -220,22 +260,22 @@ Section Process.
       | _ => False
     end.
   
-  Lemma elim_Elim :
-    forall ps qs : PidClass * (Stmt * list Context),
-      elim ps qs = true -> Elim ps qs.
-  Proof.
-    intros.
-    destruct ps as [p [ps pc]]; destruct qs as [q [qs qc]]. 
-    induction ps; destruct qs; try inversion H.
-    unfold elim in H1.
-    unfold get_stmt in H1.
-    simpl in H1.
-    destruct (eq_dec_m m m0). apply eqb_pidclass_eq in H1. subst.  
-    cbv. auto. congruence.
-    unfold elim in H. unfold get_stmt in H. simpl in H.
-    destruct (eq_dec_m m0 m). apply eqb_pidclass_eq in H. subst.
-    cbv. auto. congruence.
-  Qed.
+  (* Lemma elim_Elim : *)
+  (*   forall ps qs : PidClass * (Stmt * list Context), *)
+  (*     elim ps qs = true -> Elim ps qs. *)
+  (* Proof. *)
+  (*   intros. *)
+  (*   destruct ps as [p [ps pc]]; destruct qs as [q [qs qc]].  *)
+  (*   induction ps; destruct qs; try inversion H. *)
+  (*   unfold elim in H1. *)
+  (*   unfold get_stmt in H1. *)
+  (*   simpl in H1. *)
+  (*   destruct (eq_dec_m m m0). apply eqb_pidclass_eq in H1. subst.   *)
+  (*   cbv. auto. congruence. *)
+  (*   unfold elim in H. unfold get_stmt in H. simpl in H. *)
+  (*   destruct (eq_dec_m m0 m). apply eqb_pidclass_eq in H. subst. *)
+  (*   cbv. auto. congruence. *)
+  (* Qed. *)
     
   Definition MatchCtxt ps qt :=
     match (get_pid ps, get_pid qt, get_ctx ps, get_ctx qt) with
@@ -248,90 +288,302 @@ Section Process.
       | _ => False
     end.
   
-  Definition subst_pid p q p' :=
-    match (p, p') with
-      | (p_sng p, p_sng pid') => if eq_dec_pid p pid' then q else p'
-      | _ => p'
+  Inductive Event :=
+    | tr_skip   : Event
+    | tr_send   : PidClass -> PidClass -> T -> Event
+    | tr_choose : PidClass -> PidClass -> list (M * Stmt) -> Event
+    | tr_inst   : PidClass -> PidClass -> Event.
+  
+  Definition event_of s1 s2 :=
+    match s1, s2 with
+      | (p1, s_send _ (t,_)), (p2, s_recv _) => tr_send p1 p2 t 
+      | (p2, s_recv (t,_)), (p1, s_send _ _) => tr_send p1 p2 t 
+      | _, _ => tr_skip
     end.
   
-  Fixpoint subst_stmt p q s :=
-    match s with
-      | s_skip => s_skip
-      | s_send p' m => s_send (subst_pid p q p') (subst_pid_m p q m)
-      | s_recv m => s_recv (subst_pid_m p q m)
-      | s_seq s' t' => s_seq (subst_stmt p q s') (subst_stmt p q t')
-      | _ => s
+  Definition stitch s1 s2 :=
+    match s1, s2 with
+      | s_skip, _ => s2
+      | _, s_skip => s_skip
+      | _, _ => s_seq s1 s2
     end.
   
-  Fixpoint inst_stmt (p q : PidClass) s :=
-    match s with
-      | s_seq t u => s_seq (inst_stmt p q t) (inst_stmt p q u)
-      | s_iter xs s => s_iter xs (inst_stmt p q s)
-      | s_loop x s => s_loop x (inst_stmt p q s)
-      | s_bind x s => 
-        match (x, p) with
-          | (p_sng x', p_sng p') => 
-            if eq_dec_pid x' p' then subst_stmt p q s else s
-          | _ => s
-        end
-      | _ => s
-    end.
+  Definition dom (c : Config) := map fst c.
         
-  Inductive RewriteRel : Config -> Config -> Prop :=
+  Inductive RewriteRel : list Event -> Config -> Config -> Prop :=
   | rewrite_refl : 
       forall (c : Config), 
-        RewriteRel c c
+        RewriteRel [tr_skip] c c
 
   | rewrite_trans :
-      forall (c1 c2 c3 : Config),
-        RewriteRel c1 c2 -> RewriteRel c2 c3 ->
-        RewriteRel c1 c3
+      forall (c1 c2 c3 : Config) (t1 t2 : list Event),
+        RewriteRel t1 c1 c2 -> RewriteRel t2 c2 c3 ->
+        RewriteRel (t1 ++ t2) c1 c3
                  
   | rewrite_eq_stmt :
       forall (c : Config) (i : nat) (p : PidClass) (s t : Stmt),
         nth_config c i = Some (p, s) ->
         EqStmt s t ->
-        RewriteRel c (update_nth c i (p, t))
-
+        RewriteRel [] c (update_nth c i (p, t))
+                   
   | rewrite_bind :
-    forall (c : Config) (i : nat) (p x q : PidClass) (s t : Stmt),
+    forall (c : Config) (i : nat) (p : PidClass) (x : Var) (s s' : Stmt)
+           (t : T),
       nth_config c i = Some (p, s) ->
-      fst (head_stmt s) = s_bind x t ->
-      RewriteRel c (update_nth c i (p, inst_stmt x q s))
+      fst (head_stmt s) = s_recv_x (t, x) s' ->
+      RewriteRel [] c (update_nth c i (p, inst_stmt x (dom c) s))
                  
-  | rewrite_exit_loop :
-    forall (c : Config) (i : nat) (p : PidClass) (s t : Stmt) (X : MuVar),
-      nth_config c i = Some (p, s) ->
-      fst (head_stmt s) = s_loop X t ->
-      RewriteRel c (update_nth c i (p, s_loop_end X t))
+  (* | rewrite_exit_loop : *)
+  (*   forall (c : Config) (i : nat) (p : PidClass) (s t : Stmt) (X : MuVar), *)
+  (*     nth_config c i = Some (p, s) -> *)
+  (*     fst (head_stmt s) = s_loop X t -> *)
+  (*     RewriteRel c (update_nth c i (p, s_loop_end X t)) *)
                  
-  | rewrite_ext_choice_l :
-      forall (c : Config) (i : nat) (p : PidClass) (s t u : Stmt),
-        nth_config c i = Some (p, s) ->
-        fst (head_stmt s) = s_ext_ch t u ->
-        RewriteRel c (update_nth c i (p, update_head_stmt t s))
+  (* | rewrite_ext_choice_l : *)
+  (*     forall (c : Config) (i : nat) (p : PidClass) (s t u : Stmt), *)
+  (*       nth_config c i = Some (p, s) -> *)
+  (*       fst (head_stmt s) = s_ext_ch t u -> *)
+  (*       RewriteRel c (update_nth c i (p, update_head_stmt t s)) *)
 
-  | rewrite_ext_choice_r :
-      forall (c : Config) (i : nat) (p : PidClass) (s t u : Stmt),
-        nth_config c i = Some (p, s) ->
-        fst (head_stmt s) = s_ext_ch t u ->
-        RewriteRel c (update_nth c i (p, update_head_stmt u s))
+  (* | rewrite_ext_choice_r : *)
+  (*     forall (c : Config) (i : nat) (p : PidClass) (s t u : Stmt), *)
+  (*       nth_config c i = Some (p, s) -> *)
+  (*       fst (head_stmt s) = s_ext_ch t u -> *)
+  (*       RewriteRel c (update_nth c i (p, update_head_stmt u s)) *)
+
+  (* | rewrite_bind : *)
+  (*   forall (c : Config) (i j : nat) (p q x a : PidClass) (s t tt : Stmt), *)
+  (*     nth_config c i = Some (p, s) -> *)
+  (*     nth_config c j = Some (q, t) -> *)
+  (*     fst (head_stmt t) = s_bind x tt -> *)
+  (*     Elim (p, head_stmt s) (q, head_stmt (subst_stmt x a tt)) -> *)
+  (*     MatchCtxt (p, head_stmt s) (q, head_stmt t) -> *)
+  (*     RewriteRel [tr_choose p q] c (update_nth (update_nth c j (q, rest_stmt (inst_stmt x a t)))  *)
+  (*                                                          i (p, rest_stmt s)) *)
+
+  | rewrite_choice :
+    forall (c : Config) (i j k : nat) (p q : PidClass) (s t : Stmt) (mu : M * Stmt)
+           (ts : list (M * Stmt)),
+      nth_config c i = Some (p, s) ->
+      nth_config c j = Some (q, t) ->
+      fst (head_stmt t) = s_recv_l ts ->
+      nth_error ts k = Some mu ->
+      Elim (p, head_stmt s) (q, (s_recv (fst mu), snd (head_stmt t))) ->
+      MatchCtxt (p, head_stmt s) (q, head_stmt t) ->
+      RewriteRel [tr_choose p q ts] c 
+                 (update_nth (update_nth c j (q, update_head_stmt (snd mu) t))
+                                           i (p, rest_stmt s))
 
   | rewrite_pair :
     forall (c : Config) (i1 i2 : nat) (p1 p2 : PidClass) (s1 s2 : Stmt),
       nth_config c i1 = Some (p1, s1) -> 
       nth_config c i2 = Some (p2, s2) ->
       Elim (p1, head_stmt s1) (p2, head_stmt s2) ->
-      MatchCtxt (p1, head_stmt s1) (p2, head_stmt s2) ->
-      RewriteRel c (update_nth (update_nth c i1 (p1, rest_stmt s1)) i2 (p2, rest_stmt s2)).
-End Process.
+      MatchCtxt (p1, head_stmt s1)  (p2, head_stmt s2) ->
+      RewriteRel [event_of (p1, fst (head_stmt s1)) (p2, fst (head_stmt s2))]
+        c (update_nth (update_nth c i1 (p1, rest_stmt s1)) i2 (p2, rest_stmt s2)).
+  
+  Definition Clock := PidClass -> nat.
+  Definition ClockV := PidClass -> Clock.
 
+  Definition inc_my_clock old_cs me :=
+    fun i => if eq_dec_pidclass i me then
+               (fun them => if eq_dec_pidclass them me then 
+                              old_cs me me + 1 
+                            else 
+                              old_cs me them)
+             else
+               old_cs i.
+  
+  Definition merge_clocks (cs : ClockV) (them me : PidClass) :=
+    fun i => if eq_dec_pidclass i me then
+               (fun c => PeanoNat.Nat.max
+                           (cs them c) (cs me c))
+             else
+               cs i.
+
+  Fixpoint run_clock (cs : ClockV) (es : list Event) :=
+    match es with
+      | nil => nil
+      | tr_send a b t :: es' => 
+        (tr_send a b t, cs) ::
+        run_clock (merge_clocks (inc_my_clock (inc_my_clock cs a) b) a b) es'
+      | tr_choose a b ss :: es' => 
+        (tr_choose a b ss, cs) ::
+        run_clock (merge_clocks (inc_my_clock (inc_my_clock cs a) b) a b) es'
+      | _ :: es' => 
+        run_clock cs es'
+    end.
+  
+  Definition ClocksLt (cs cs' : ClockV) (i j : PidClass) :=
+    (forall x, cs i x <= cs' j x) /\ (exists x, cs i x < cs' j x).
+  
+  Definition Overlap (x y : list M) := False.
+  
+  Definition NoRaces (e : (Event * ClockV)) (es : list (Event * ClockV)) :=
+    Forall (fun e' => 
+              match fst e, fst e' with
+                | tr_choose a b s, tr_choose a' b' s' =>
+                  a <> a' /\ b = b' /\
+                  map snd s <> map snd s' /\
+                  Overlap (map fst s) (map fst s')
+                  -> ClocksLt (snd e) (snd e') a a'
+                | _,_ => True
+              end) es.
+ 
+  (* Definition find_races (e : Event) (es : list (Event * ClockV)) := *)
+  (*   fst (partition (fun x =>  *)
+  (*                     match e, fst x with *)
+  (*                       | tr_choose a b s, tr_choose a' b' s' => *)
+  (*                         a <> a' /\ b = b' /\ *)
+  (*                         map snd s <> map snd s' /\ *)
+  (*                         Overlap (map fst s) (map fst s') *)
+  (*                    | _, _ => false *)
+  (*                  end) es). *)
+  
+  (* Definition CheckE ec1 ec2 := *)
+  (*   match fst ec1, fst ec2 with *)
+  (*     | tr_inst a _, tr_inst b _ => ClocksLt (snd ec1) (snd ec2) a b *)
+  (*     | _,_ => True *)
+  (*   end. *)
+   
+  Fixpoint Causal' (es : list (Event * ClockV)) :=
+    match es with
+      | [] => True
+      | ec :: es' => NoRaces ec es' /\ Causal' es'
+      (* | ec :: es' => match find_races (fst ec) es' with *)
+      (*                  | [] => Causal' es' *)
+      (*                  | es => fold_left (fun p ec' => p /\ CheckE ec ec') es (Causal' es') *)
+                     (* end *)
+    end.
+  
+  Definition Causal t := Causal' (run_clock (fun _ _ => 0) t).
+ 
+  (* Parameter t : T. *)
+
+  (* Definition x :=  (run_clock (fun _ => fun _ => 0)  *)
+  (*                 [tr_send (p_sng 0) (p_sng 2) t;  *)
+  (*                   tr_send (p_sng 0) (p_sng 1) t;  *)
+  (*                   tr_send (p_sng 2) (p_sng 1) t]) : list (Event * (PidClass -> PidClass -> nat))%type. *)
+  
+  (* Ltac simpl_clocks := *)
+  (*   repeat (cbn; match goal with  *)
+  (*     | |- context[eq_dec_pidclass ?x ?x] => destruct (eq_dec_pidclass x x); [ idtac | congruence ] *)
+  (*     | |- context[eq_dec_pidclass ?x ?y] => destruct (eq_dec_pidclass x y); [ congruence | idtac ] *)
+  (*     | |- context[eq_dec_pidclass ?x ?y] => destruct (eq_dec_pidclass x y)  *)
+  (*     | |- context[merge_clocks] => unfold merge_clocks at 1 *)
+  (*     | |- context[inc_my_clock] => unfold inc_my_clock at 1 *)
+  (*   end); try solve [cbv; auto]. *)
+  
+  (* Goal (Causal x). *)
+  (*   Proof.  *)
+  (*     intros. *)
+  (*     simpl. *)
+  (*     destruct (eq_dec_T t t); [ idtac | congruence ]. *)
+  (*     unfold ClocksLt. *)
+  (*     repeat split. *)
+  (*     intros. *)
+  (*     simpl_clocks. *)
+  (*     simpl_clocks. *)
+  (*     eapply ex_intro. *)
+
+  (* Goal match (tl (tl x)) with *)
+  (*        | (_, f)::_ => f (p_sng 1) (p_sng 1) = 2 *)
+  (*        | _ => True *)
+  (*      end. *)
+  (* Proof. simpl_clocks. Qed. *)
+  
+  (* Definition c1 := (inc_my_clock (inc_my_clock (fun _ _ => 0) (p_sng 0)) (p_sng 1)). *)
+  (* Definition c2 := (inc_my_clock (inc_my_clock (fun _ _ => 0) (p_sng 1)) (p_sng 1)). *)
+  
+  (* Goal  *)
+  (*   forall (i : PidClass), *)
+  (*     c2 (p_sng 0) i <= c1 (p_sng 1) i. *)
+  (* Proof. *)
+  (*   intros. *)
+  (*   unfold c1, c2. *)
+  (*   simpl_clocks.  *)
+  (* Qed. *)
+
+(* Fixpoint first_st (f : Trace -> bool) (l : list Trace) := *)
+(*   match l with *)
+(*     | [] => ([], None) *)
+(*     | h::t => if f h then *)
+(*                 ([], Some h) *)
+(*               else *)
+(*                 match first_st f t with *)
+(*                   | (l', xo) => (h :: l', xo) *)
+(*                 end *)
+(*   end. *)
+
+(* Definition Linear' (t : Trace) (ts : list Trace) : Prop := *)
+(*   match t with *)
+(*     | tr_send a b t => *)
+(*       match first_st (fun x => match x with *)
+(*                                  | tr_send a' b' t' => *)
+(*                                    andb (negb (eqb_pidclass a a')) *)
+(*                                         (andb (eqb_pidclass b b') *)
+(*                                               (if eq_dec_T t t' then true else false)) *)
+(*                                  | _ => false *)
+(*                                end) ts with *)
+(*         | (_, None) => True *)
+(*         | (ls, Some t') => True *)
+(*       end *)
+(*     | _ => True *)
+(*   end. *)
+
+(* Inductive prefix : Trace -> Trace -> list Trace -> Prop := *)
+(* | prefix_in : *)
+(*     forall t1 t2 ts ts', *)
+(*       In t1 ts -> In t2 ts' -> prefix t1 t2 (ts ++ ts'). *)
+
+(* Inductive prefix_II_IO_chain : Trace -> Trace -> list Trace -> Prop := *)
+(* | IO_end :  *)
+(*     forall (p q : PidClass) (t : T) *)
+(*            prefix *)
+      
+(* | II_IO_chain : *)
+(*     forall t1 t2  *)
+
+
+(* Fixpoint Linear (t : list Trace) : Prop := *)
+(*   match t with *)
+(*     | [] => True *)
+(*     | t::ts => Linear' t ts /\ Linear ts *)
+(*   end. *)
+  
+
+(* Axiom linear_skip_1 : forall (t : list Trace), *)
+(*                       Linear (tr_skip::t) <-> Linear t. *)
+(* Axiom linear_skip_2 : forall (t : list Trace), *)
+(*                       Linear (t ++ [tr_skip]) <-> Linear t. *)
+
+Fixpoint seq_stmts ss :=
+  match ss with
+    | []%list => s_skip
+    | s::nil => s
+    | (s::ss) => s_seq s (seq_stmts ss)
+  end.
+
+Definition seq s1 s2 :=
+  match s2 with 
+    | s_skip => s1
+    | _ => s_seq s1 s2
+  end.
+End Process.
 Hint Constructors RewriteRel : rewrite.
 
-Notation "[ x ]" := (cons x nil).
-Notation "[ x | .. | y ]" := (cons x .. (cons y nil) ..).
-Notation "P1 ; P2" := (s_seq P1 P2) (at level 65, right associativity).
-Notation "P [[ S ]]" := (p_sng P, S) (at level 80).
-Notation "{ P } [[ S ]]" := (p_set P, S) (at level 80).
-Notation "C1 ===> C2" := (RewriteRel C1 C2) (at level 95).
-Notation "X ~ S" := (s_bind (p_sng X) S) (at level 60).
+Local Close Scope list.
+Delimit Scope config_scope with config.
+(* Notation "[ x ]" := (cons x nil) : config. *)
+(* Notation "[ x | .. | y ]" := (cons x .. (cons y nil) ..) : config. *)
+
+Delimit Scope stmt_scope with stmt.
+
+Notation "[[ S1 ]]" := (S1) : stmt.
+Notation "[[ S1 ; .. ; S2 ]]" := (seq S1 .. (seq S2 s_skip) ..) : stmt.
+Notation "P @ S" := (p_sng P, S) (at level 80).
+Notation "{ P } @ S " := (p_set P, S) (at level 80).
+Notation "C1 ===> C2 + T " := (RewriteRel T C1 C2) (at level 95).
+Notation "C1 ===> C2 " := (exists T, RewriteRel T C1 C2 /\ Causal T) (at level 95).
+Notation "X ~ recv( T ) S" := (s_recv_x (X, T) S) (at level 60).
