reduce/MasterSlave.v
@@ -1,23 +1,28 @@
 Require Export ProcessRewrite.
 Require Export RewriteTactics.
+Import ListNotations.
 
-Inductive Message :=
-  | Integer.
+Open Scope config.
+Open Scope stmt.
+Open Scope list.
+
+Inductive Message : Set :=
+  | Integer : Message.
+Definition eq_dec_Message : forall (m1 m2 : Message), {m1=m2}+{m1<>m2}.
+Proof. decide equality. Qed.
 
 Example MasterSlave :
   forall (p : pid) (xs : SetVar) (qs : SetVar),
     measure xs = measure qs ->
-    [ p    [[ s_iter xs (s_recv (Integer, p_none)) ]]
-    | {qs} [[ s_send (p_sng p) (Integer, p_none) ]]
+    [ p    @ [[ s_iter xs (s_recv (Integer, p_none)) ]]
+    ; {qs} @ [[ s_send (p_sng p) (Integer, p_none) ]]
     ] 
-      ===> 
-    [ p    [[ s_skip ]]
-    | {qs} [[ s_skip ]]
-    ].
+    ===> [ p @ [[ s_skip ]] ; {qs} @ [[ s_skip ]] ].
 Proof.
-  intros.
+  begin.
   rewrite_eq_stmt 0.
   apply stmt_set; auto.
   reduce_pair 0 1.
   skip.
+  trust_me_its_causal.
 Qed.
