reduce/PingMany.v
@@ -1,25 +1,29 @@
 Require Export ProcessRewrite.
 Require Export RewriteTactics.
+Import ListNotations.
 
 Inductive PingPong :=
 | Ping : PingPong
 | Pong : PingPong.
 
+Open Scope config.
+Open Scope stmt.
+Open Scope list.
+
 Example PingPong_many :
-  forall (q x : nat) (ps : SetVar),
-    q <> x ->
-    [ { ps } [[ s_send (p_sng q) (Ping, p_set ps); x ~ (s_recv (Pong, p_sng x)) ]]
-    |   q    [[ s_iter ps
-                 (x ~ (s_recv (Ping, p_sng x); 
-                       s_send (p_sng x) (Pong, p_sng q)))]] 
-    ] ===> [ { ps } [[ s_skip ]] 
-           | q [[ s_skip ]] 
-           ].
+  forall (q : nat) (x ps : Var),
+     ( [ { ps } @ [[ s_send (p_sng q) (tt, p_set ps); 
+                     s_recv_x (tt,x) s_skip ]]
+       ; q      @ [[ s_iter ps
+                   (s_recv_x (tt,x) (s_send (p_var x) (tt, p_sng q))) ]]
+      ] ===>
+      [ { ps } @ s_skip ; q @ s_skip ]).
 Proof.
-  intros.
-  inst_bind 1.
-  reduce_pair 0 1.
+  begin.
+  inst_bind 1. 
+  reduce_choice 0 1 0.
   inst_bind 0.
-  reduce_pair 0 1.
+  reduce_choice 1 0 1.
   skip.
+  trust_me_its_causal.
 Qed.
