reduce/RacySend.v
@@ -1,0 +1,148 @@
+Require Export ProcessRewrite.
+Require Export RewriteTactics.
+
+Inductive Message :=
+  | t1 | t2 | t3.
+
+Parameter x y p q r : nat.
+
+Definition p_proc :=
+  s_send (p_sng q) (t1, p_sng p); s_recv (t2, p_none).
+
+Definition q_proc :=
+  s_bind (p_sng x) (s_recv (t1, p_sng x); s_send (p_sng x) (t2, p_none);
+            (s_bind (p_sng y) (s_recv (t1, p_sng y); s_send (p_sng y) (t3, p_none)))).
+
+Definition r_proc :=
+  s_send (p_sng q) (t1, p_sng r); s_recv (t3, p_none).
+
+  Ltac simpl_clocks :=
+    repeat (match goal with
+      | |- context[eq_dec_pidclass ?x ?x] => destruct (eq_dec_pidclass x x); [ idtac | congruence ]
+      | |- context[eq_dec_pidclass ?x ?y] => destruct (eq_dec_pidclass x y); [ congruence | idtac ]
+      | |- context[eq_dec_pidclass ?x ?y] => destruct (eq_dec_pidclass x y)
+      | |- context[inc_my_clock] => unfold inc_my_clock at 1
+      | |- context[merge_clocks] => unfold merge_clocks at 1
+    end); cbn.
+
+  Ltac simpl_clocks_h :=
+    repeat (match goal with
+      | H : context[eq_dec_pidclass ?x ?x] |- _ => destruct (eq_dec_pidclass x x); [ idtac | congruence ]
+      | H : context[eq_dec_pidclass ?x ?y] |- _=> destruct (eq_dec_pidclass x y); [ congruence | idtac ]
+      | H : context[eq_dec_pidclass ?x ?y] |- _ => destruct (eq_dec_pidclass x y)
+      | H : context[inc_my_clock] |- _ => unfold inc_my_clock at 1 in H
+      | H : context[merge_clocks] |- _ => unfold merge_clocks at 1 in H
+    end); cbn.
+
+Example bad :
+  x <> y -> 
+  x <> p -> x <> q -> x <> r ->
+  y <> p -> y <> q -> y <> r ->
+  p <> q -> p <> r -> q <> r -> 
+  (exists t,
+    RewriteRel t 
+               [ p [[ p_proc ]] | q [[ q_proc ]] | r [[ r_proc ]] ]
+               [ p [[ s_skip ]] | q [[ s_skip ]] | r [[ s_skip ]] ]
+    /\ (~ Causal t)).
+Proof.
+  intros.
+  eapply ex_intro.
+  split.
+  unfold p_proc, q_proc, r_proc.
+  inst_bind 0 1.
+  reduce_pair 0 1.
+  inst_bind 2 1.
+  reduce_pair 2 1.
+  skip.
+  simpl Causal.
+  unfold Causal, run_clock, Causal', find_races, partition.
+  simpl partition. simpl fst.
+  match goal with
+    | |- context[if (?b : bool) then _ else _]  => destruct b eqn:X; cbn
+  end.
+  intro.
+  destruct H9.
+  unfold ClocksLt in H10.
+  destruct H10.
+  destruct H11.
+  simpl_clocks_h. inversion H11.
+  unfold andb in X.
+  unfold negb in X.
+  destruct H7.
+  destruct (Nat.eqb p r) eqn:Y.
+  rewrite PeanoNat.Nat.eqb_eq in *.
+  assumption.
+  destruct X. 
+  rewrite <- PeanoNat.Nat.eqb_eq in *.
+  rewrite Y.
+  apply PeanoNat.Nat.eqb_eq. reflexivity.
+Qed.
+
+  unfold merge_clocks at 1 in H11.
+  destruct (eq_dec_pidclass (p_sng r) (p_sng p)); [ congruence | idtac ].
+  
+  split; auto.
+  unfold ClocksLt.
+  split.
+  intros.
+  simpl_clocks.
+  auto.
+  exists (p_sng r); simpl_clocks.
+  ex_intro.
+  simpl_clocks.
+  
+  unfold run_clock.
+  find_races, partition.
+ 
+  simpl event_of.
+  simpl app.
+  unfold Causal.
+  simpl run_clock.
+  cbn.
+  unfold find_races.
+  unfold partition.
+  cbn.
+  destruct (negb (Nat.eqb p r) && Nat.eqb q q)%bool. 
+  simpl. split.
+  unfold inc_my_clock at 1.
+  unfold inc_my_clock.
+  simpl.
+  simpl.
+  unfold find_races.
+  unfold partition.
+ repeat (match goal with
+      (* | |- context[eq_dec_pidclass ?x ?x] => destruct (eq_dec_pidclass x x); [ idtac | congruence ] *)
+      (* | |- context[eq_dec_pidclass ?x ?y] => destruct (eq_dec_pidclass x y); [ congruence | idtac ] *)
+      | |- context[eq_dec_pidclass ?x ?y] => destruct (eq_dec_pidclass x y)
+      | |- context[inc_my_clock] => unfold inc_my_clock at 1
+      (* | |- context[merge_clocks] => unfold merge_clocks at 1 *)
+    end).
+
+  unfold inc_my_clock at 6.
+  cbn.
+  Ltac t H :=
+    match H with
+      | context G [inc_my_clock] => t G
+      | _ => unfold inc_my_clock at 1
+      (* | |- context[inc_my_clock] => t G *)
+    end.
+  match goal with
+    | |- context H [inc_my_clock] => 
+      let x := context H [inc_my_clock] in
+      t x
+  end.
+ repeat (match goal with
+      | |- context[eq_dec_pidclass ?x ?x] => destruct (eq_dec_pidclass x x); [ idtac | congruence ]
+      | |- context[eq_dec_pidclass ?x ?y] => destruct (eq_dec_pidclass x y); [ congruence | idtac ]
+      (* | |- context[eq_dec_pidclass ?x ?y] => destruct (eq_dec_pidclass x y) *)
+      | |- context[inc_my_clock] => unfold inc_my_clock at 1
+      (* | |- context[merge_clocks] => unfold merge_clocks at 1 *)
+    end).
+
+  simpl_clocks.
+  unfold inc_my_clock at 1.
+  unfold inc_my_clock at 1.
+  simpl_clocks.
+  unfold merge_clocks at 1. 
+  destruct (eq_dec_pidclass
+  simpl_clocks.
