reduce/RewriteTactics.v
@@ -1,8 +1,17 @@
 Require Export ProcessRewrite.
+Import ListNotations.
+Require Import PeanoNat.
+Require Import Nat.
+Require Import Bool.
 
 Hint Constructors EqStmt : eqstmt.
 
+Ltac begin := intros; eapply ex_intro; split.
 Ltac skip := solve[apply rewrite_refl].
+
+Open Scope stmt.
+Open Scope list.
+Open Scope config.
 
 Ltac rewrite_eq_stmt x :=
   eapply rewrite_trans; 
@@ -13,26 +22,92 @@ Ltac reduce_pair i j :=
   eapply rewrite_trans;
     [apply rewrite_pair with (i1 := i) (i2 := j); try reflexivity | idtac]; cbv; auto.
 
-Ltac expand_subst :=
+Lemma break_if_pidclass :
+  forall (x : PidClass), 
+    eqb_pidclass x x = false -> False.
+Proof.
+  intro.
+  unfold eqb_pidclass.
+  destruct x; 
+  try rewrite Nat.eqb_refl in *; intuition.
+  destruct v. 
+  unfold eqb_var in *.
+  try rewrite Nat.eqb_refl in *; intuition.
+  destruct v. 
+  unfold eqb_var in *.
+  try rewrite Nat.eqb_refl in *; intuition.
+Qed.
+
+Lemma break_if_pidclass_neg :
+  forall (x y : PidClass), 
+    x <> y ->
+    eqb_pidclass x y = true -> False.
+Proof.
+  intro.
+  unfold eqb_pidclass.
+  destruct x; destruct y;
+  try rewrite Nat.eqb_refl in *; intuition.
+  apply H.
+  f_equal.
+  rewrite <- Nat.eqb_eq.
+  exact H0.
+  destruct v; destruct v0. 
+  apply H.
+  repeat f_equal.
+  rewrite <- Nat.eqb_eq.
+  exact H0.
+  destruct v; destruct v0. 
+  apply H.
+  repeat f_equal.
+  rewrite <- Nat.eqb_eq.
+  exact H0.
+Qed.
+
+Ltac kill_substs :=
   simpl; simpl inst_stmt; simpl subst_stmt; unfold subst_pid_m, subst_pid;
-    repeat match goal with
-             | |- context[eq_dec_pid ?x ?x] =>
-               destruct (eq_dec_pid x x); [ idtac | congruence]
-             | |- context[eq_dec_pid ?x ?y] =>
-               destruct (eq_dec_pid x y); [ congruence | idtac]
-           end.
+ repeat (
+     match goal with
+       | |- context[eqb_pidclass ?x ?x] =>
+         let H := fresh "Kill_eqb" in
+         destruct (eqb_pidclass x x) eqn: H; [ auto | 
+          exfalso; eauto using break_if_pidclass]; clear H
+     end
+   ).
+
+Ltac defeat_eqs :=
+  match goal with
+    | |- context[eq_dec_pid ?x ?x] => destruct (eq_dec_pid x x); [ auto | congruence ]; cbn
+    | |- context[eq_dec_pid ?x ?y] => destruct (eq_dec_pid x y); [ congruence | auto ]; cbn
+  end.
 
 Ltac inst_bind x :=
-  eapply rewrite_trans; [
-      eapply rewrite_bind with (i := x)
-    | idtac ]; simpl; try reflexivity; expand_subst.
+  eapply rewrite_trans;
+    [eapply rewrite_bind with (i := x); cbn; try reflexivity | idtac]; 
+    cbn; auto; kill_substs.
 
-Ltac choose_left x :=
+Ltac reduce_choice x y z :=
   eapply rewrite_trans; 
-  [ eapply rewrite_ext_choice_l with (i := x); try reflexivity | idtac];
-  simpl. 
+  [ eapply rewrite_choice with (i := x) (j := y) (k := z); cbv | idtac ]; try reflexivity; cbv; auto.
 
-Ltac choose_right x :=
-  eapply rewrite_trans; 
-  [ eapply rewrite_ext_choice_r with (i := x); try reflexivity | idtac];
-  simpl. 
+(* Ltac choose_left x := *)
+(*   eapply rewrite_trans;  *)
+(*   [ eapply rewrite_ext_choice_l with (i := x); try reflexivity | idtac]; *)
+(*   simpl.  *)
+
+(* Ltac choose_right x := *)
+(*   eapply rewrite_trans;  *)
+(*   [ eapply rewrite_ext_choice_r with (i := x); try reflexivity | idtac]; *)
+(*   simpl.  *)
+
+Ltac trust_me_its_causal :=
+  unfold Causal, Causal', NoRaces; cbn;
+  repeat ( 
+      match goal with
+        | H : @In _ _ [] |- _ => inversion H
+        | H : _ /\ _ |- _ => decompose [and or] H; clear H
+        | H : @In _ _ _ |- _ =>
+          apply in_inv in H; destruct H; subst; cbn; intros
+        | |- context[Forall _ _]  =>
+          rewrite Forall_forall; split; intros
+      end; try congruence
+    ); auto.
